The theories in examples/elliptic/sep are now up-to-date with the latest version of Anthony's theories in examples/elliptic/arm.

examples/elliptic/sep/arm_progLib.sig
@@ -6,6 +6,9 @@ sig
 
     val dest_ARM_PROG       : term -> term * term * term * term * term   
 
+    val FST_PROG2           : thm -> thm
+    val SND_PROG2           : thm -> thm
+
     val ARM_PROG_PRE_CONV   : conv -> conv   
     val ARM_PROG_POST1_CONV : conv -> conv
     val ARM_PROG_POST_CONV  : conv -> conv
@@ -21,6 +24,7 @@ sig
     val pcINC_ss            : simpLib.ssfrag
     val setINC_ss           : simpLib.ssfrag
     val compose_ss          : simpLib.ssfrag
+    val armINST_ss          : simpLib.ssfrag
 
     val MATCH_COMPOSE       : thm -> thm -> thm
     val ARRANGE_COMPOSE     : thm -> thm -> thm
@@ -30,6 +34,10 @@ sig
     val HIDE_POST1          : thm -> thm
     val HIDE_POST           : thm -> thm
     val HIDE_STATUS         : thm -> thm
+
+    val AUTO_PRE_HIDE_STATUS   : thm -> thm
+    val AUTO_POST1_HIDE_STATUS : thm -> thm
+    val AUTO_POST_HIDE_STATUS  : thm -> thm
 
     val APP_BASIC_FRAME     : thm -> thm
     val APP_FRAME           : term frag list -> thm -> thm
@@ -49,8 +57,16 @@ sig
     val APP_PART_WEAKEN_TERM     : thm -> term frag list -> term 
     val APP_PART_WEAKEN          : thm -> term frag list -> tactic -> thm 
 
+    val ALIGN_VARS          : string list -> thm -> thm
+
     val PAT_DISCH           : term -> thm -> thm
     val PAIR_GEN            : string -> term frag list -> thm -> thm
+
+    val show_enc            : bool ref
+    val show_code           : bool ref
+    val show_code_verbosely : bool ref
+ 
+    val pp_enc              : unit -> unit
 
     (* experimental proof-producing functions *)
  
